Coq formalization

Verif_levenshtein.v
@@ -1,91 +1,101 @@
 Require Import Coq.Strings.String.
 Require Import Coq.Strings.Ascii.
+Require Import Coq.Lists.List.
 Require Import Coq.Init.Peano.
 Require Import Omega.
 Require Import Coq.Program.Equality.
 
-Definition insert (i : nat) (c : ascii) (s : string) : string :=
-  substring 0 i s ++ String c EmptyString ++ substring i (length s) s.
-Definition delete (i : nat) (s : string) : string :=
-  substring 0 i s ++ substring (S i) (length s) s.
-Definition update (i : nat) (c : ascii) (s : string) : string :=
-  substring 0 i s ++ String c EmptyString ++ substring (S i) (length s) s.
+Definition lstring := list ascii.
 
-Eval compute in (substring 1 2 "a").
-Eval compute in (insert 1 "!" "joomy").
-Eval compute in (delete 6 "joomy").
-Eval compute in (update 0 "J" "joomy").
+Section Isomorphism.
 
-Inductive edit : string -> string -> Type :=
-| insertion (i : nat) (c : ascii) (s : string) : edit s (insert i c s)
-| deletion (i : nat) (s : string) : edit s (delete i s)
-| substitution (i : nat) (c : ascii) (s : string) : edit s (update i c s).
+Fixpoint to_string (l : lstring) : string :=
+  match l with
+  | nil => EmptyString
+  | cons x xs => String x (to_string xs)
+  end.
+Fixpoint to_lstring (s : string) : lstring :=
+  match s with
+  | EmptyString => nil
+  | String x xs => cons x (to_lstring xs)
+  end.
+Lemma lstring_same : forall l, to_lstring (to_string l) = l.
+Proof. intro l; induction l; simpl; f_equal; auto. Defined.
 
-Inductive chain : string -> string -> Type :=
+Lemma string_same : forall s, to_string (to_lstring s) = s.
+Proof. intro s; induction s; simpl; f_equal; auto. Defined.
+
+Definition on_string (f : lstring -> lstring) (s : string) : string :=
+  to_string (f (to_lstring s)).
+Definition on_lstring (f : string -> string) (l : lstring) : lstring :=
+  to_lstring (f (to_string l)).
+
+End Isomorphism.
+
+Open Scope list_scope.
+Import ListNotations.
+
+Definition insert (i : nat) (c : ascii) (s : lstring) : lstring :=
+  firstn i s ++ [c] ++ skipn i s.
+Definition delete (i : nat) (s : lstring) : lstring :=
+  firstn i s ++ skipn (S i) s.
+Definition update (i : nat) (c : ascii) (s : lstring) : lstring :=
+  firstn i s ++ [c] ++ skipn (S i) s.
+
+Eval compute in (on_string (insert 1 "!") "joomy").
+Eval compute in (on_string (delete 1) "joomy").
+Eval compute in (on_string (update 0 "J") "joomy").
+
+Inductive edit : lstring -> lstring -> Type :=
+| insertion (i : nat) (c : ascii) (s : lstring) : edit s (insert i c s)
+| deletion (i : nat) (s : lstring) : edit s (delete i s)
+| substitution (i : nat) (c : ascii) (s : lstring) : edit s (update i c s).
+
+Inductive chain : lstring -> lstring -> Type :=
 | same : forall s, chain s s
 | change : forall s s' t, edit s s' -> chain s' t -> chain s t.
 
-Fixpoint chain_length {s t : string} (c : chain s t) : nat :=
+Fixpoint chain_length {s t : lstring} (c : chain s t) : nat :=
   match c with
   | same _ => 0
   | change _ _ _ _ c' => chain_length c'
   end.
 
-Lemma substring_same : forall i s, substring i i s = EmptyString.
-(* intros i s. *)
-(* induction s. *)
-(* simpl in *. destruct i; auto. *)
-(* generalize dependent s. *)
-Admitted.
-
-
-Lemma substring_more : forall i s, i >= length s -> substring 0 i s = s.
-Admitted.
-
-Lemma substring_all : forall s, substring 0 (length s) s = s.
-Proof. intros. apply substring_more. auto. Qed.
-
-Lemma substring_append : forall s i j k, substring i k = substring i j ++ substring j k.
-
-Lemma weaken_edit (a : ascii) (s1 s2 : string) (e : edit s1 s2) : edit (String a s1) (String a s2).
-Proof.
+Lemma weaken_edit (a : ascii) (s1 s2 : lstring) (e : edit s1 s2) : edit (cons a s1) (cons a s2).
 inversion e.
-* subst.
-  pose (insertion (S i) c (String a s1)) as e'.
-  unfold insert in *.
-  simpl in *.
-  rewrite (substring_more (S (length s1)) s1) in e'.
+* pose (insertion (S i) c (cons a s1)). auto.
+* pose (deletion (S i) (cons a s1)). auto.
+* pose (substitution (S i) c (cons a s1)). auto.
+Qed.
 
-
-
-Lemma insert_chain : forall c s1 s2, chain s1 s2 -> chain s1 (String c s2).
+Lemma insert_chain : forall c s1 s2, chain s1 s2 -> chain s1 (cons c s2).
 intros.
-apply (change _ (String c s1)).
+apply (change _ (cons c s1)).
 pose (insertion 0 c s1) as e.
-unfold insert in e.
-rewrite (substring_same 0 s1) in e.
-rewrite (substring_all s1) in e.
 auto.
+induction H.
 constructor.
-Defined.
+pose (weaken_edit c s s' e) as e'.
+apply (change _ _ _ e' IHchain).
+Qed.
 
 Lemma inserts_chain : forall s1 s2, chain s2 (s1 ++ s2).
 intros.
 induction s1; simpl.
 constructor.
-
 apply insert_chain.
+auto.
+Qed.
 
-Admitted.
-
-Lemma delete_chain : forall c s, chain (String c s) s.
+Lemma delete_chain : forall c s, chain (cons c s) s.
 intros.
 apply (change _ s).
-pose (deletion 0 (String c s)) as e.
+pose (deletion 0 (cons c s)) as e.
 unfold delete in *.
 simpl in e.
-Admitted.
+auto.
+constructor.
+Qed.
 
-
-Fixpoint levenshtein_chain (s t : string) : chain s t.
+Fixpoint levenshtein_chain (s t : lstring) : chain s t.
 Admitted.
